Add simple coupon induction rules

eqqq.thy
@@ -85,46 +85,14 @@ datatype step_result =
   Continue state
   | Return handle
 
-inductive step :: "op \<Rightarrow> state \<Rightarrow> step_result \<Rightarrow> bool"
-  where
-    StepGetBlobData:
-    "i < length (hs s) \<Longrightarrow> hs s ! i = HBlobHandle b \<Longrightarrow>
-    step (OGetBlobData i) s (Continue (dpush s (get_blob_data b)))"
-
-| StepGetTreeData:
-  "i < length (hs s) \<Longrightarrow> 
-     hs s ! i = HTreeHandle t \<Longrightarrow>
-     j < get_tree_size t \<Longrightarrow>
-    step (OGetTreeData i j) s (Continue (hpush s (get_tree_data t j)))"
-
-| StepCreateBlob:
-  "i < length (ds s) \<Longrightarrow> 
-    step (OCreateBlob i) s (Continue (hpush s (HBlobHandle (create_blob (ds s ! i)))))"
-
-| StepCreateThunk:
-  "i < length (hs s) \<Longrightarrow> hs s ! i = HTreeHandle t \<Longrightarrow>
-    step (OCreateThunk i) s (Continue (hpush s (HThunkHandle (create_thunk t))))"
-
-| StepCreateTree:
-  "\<forall>i\<in>set xs. i < length (hs s) \<Longrightarrow>
-     hlist = map (\<lambda>i. hs s ! i) xs \<Longrightarrow>
-     step (OCreateTree xs) s (Continue (hpush s (HTreeHandle (create_tree hlist) )))" 
-
-| StepReturn:
-  "i < length (hs s) \<Longrightarrow> r = hs s ! i \<Longrightarrow>
-    step (OReturn i) s (Return (hs s ! i))"
-
-| StepRunInternal:
-  "step ORunInternal s (Continue (run_internal s))"
-
-fun step_fun :: "op \<Rightarrow> state \<Rightarrow> step_result option" where
-  "step_fun (OGetBlobData i) s = 
+fun step :: "op \<Rightarrow> state \<Rightarrow> step_result option" where
+  "step (OGetBlobData i) s = 
       (if i < length (hs s) then
          (case (hs s ! i) of
           HBlobHandle b \<Rightarrow> Some (Continue (dpush s (get_blob_data b)))
         | _ \<Rightarrow> None)
        else None)"
-| "step_fun (OGetTreeData i j) s =
+| "step (OGetTreeData i j) s =
       (if i < length (hs s) then
          (case (hs s ! i) of
           HTreeHandle t \<Rightarrow> (if (j < get_tree_size t) 
@@ -132,181 +100,66 @@ fun step_fun :: "op \<Rightarrow> state \<Rightarrow> step_result option" where
                             else None)
           | _ \<Rightarrow> None)
        else None)"
-| "step_fun (OCreateBlob i) s =
+| "step (OCreateBlob i) s =
       (if i < length (ds s) then
          Some (Continue (hpush s (HBlobHandle (create_blob (ds s ! i)))))
        else None)"
-| "step_fun (OCreateThunk i) s =
+| "step (OCreateThunk i) s =
       (if i < length (hs s) then
          case (hs s ! i) of
          HTreeHandle t \<Rightarrow> Some (Continue (hpush s (HThunkHandle (create_thunk t))))
          | _ \<Rightarrow> None
        else None)"
-| "step_fun (OCreateTree xs) s =
+| "step (OCreateTree xs) s =
       (if (\<forall>i\<in>set xs. i < length (hs s)) then
         (let hlist = map (\<lambda>i. hs s ! i) xs in
          Some (Continue (hpush s (HTreeHandle (create_tree hlist)))))
       else None)"
-| "step_fun (OReturn i) s =
+| "step (OReturn i) s =
       (if i < length (hs s) then Some (Return (hs s ! i)) else None)"
-| "step_fun (ORunInternal) s = Some (Continue (run_internal s))"
+| "step (ORunInternal) s = Some (Continue (run_internal s))"
 
-inductive exec :: "userprog \<Rightarrow> state \<Rightarrow> handle \<Rightarrow> bool"
+fun exec :: "userprog \<Rightarrow> state \<Rightarrow> handle option"
   where
-    ExecReturn:
-    "step i s (Return r) \<Longrightarrow> exec (i # xs) s r"
-  | ExecStep:
-    "step i s (Continue s') \<Longrightarrow> exec xs s' r \<Longrightarrow> exec (i # xs) s r"
-
-fun exec_fun :: "userprog \<Rightarrow> state \<Rightarrow> handle option"
-  where
-    "exec_fun [] s = None"
-  | "exec_fun (i # xs) s =
-   (case (step_fun i s) of
+    "exec [] s = None"
+  | "exec (i # xs) s =
+   (case (step i s) of
    None \<Rightarrow> None
    | Some (Return r) \<Rightarrow> Some r
-   | Some (Continue s') \<Rightarrow> exec_fun xs s')"
+   | Some (Continue s') \<Rightarrow> exec xs s')"
 
 (* Thunk evaluation *)
 
 definition state_init :: "ThunkHandle \<Rightarrow> state" where
   "state_init thunk \<equiv> \<lparr> hs = [HTreeHandle (get_thunk_tree thunk)], ds = [] \<rparr>"
 
-definition apply_thunk :: "ThunkHandle \<Rightarrow> handle option" where
-  "apply_thunk th \<equiv> exec_fun (get_prog (get_thunk_tree th)) (state_init th)" 
+definition think :: "ThunkHandle \<Rightarrow> handle option" where
+  "think th \<equiv> exec (get_prog (get_thunk_tree th)) (state_init th)" 
 
 fun is_thunk :: "handle \<Rightarrow> bool" where
   "is_thunk (HThunkHandle _) = True"
 | "is_thunk _ = False"
 
-inductive force_with_fuel :: "nat \<Rightarrow> handle \<Rightarrow> handle \<Rightarrow> bool" where
-  Done:
-  "\<not> is_thunk h \<Longrightarrow> force_with_fuel n h h"
-| Step:
-  "h = HThunkHandle thunk \<Longrightarrow>
-     Some h1 = apply_thunk thunk \<Longrightarrow>
-     force_with_fuel n h1 h2 \<Longrightarrow>
-     force_with_fuel (Suc n) h h2"
-
-fun force_with_fuel_fun :: "nat \<Rightarrow> handle \<Rightarrow> handle option" where
-  "force_with_fuel_fun n h =
+fun force_with_fuel :: "nat \<Rightarrow> handle \<Rightarrow> handle option" where
+  "force_with_fuel n h =
      (case h of
         HThunkHandle th \<Rightarrow>
           (case n of
              0 \<Rightarrow> None
            | Suc n' \<Rightarrow>
-               (case apply_thunk th of
+               (case think th of
                   None \<Rightarrow> None
-                | Some h1 \<Rightarrow> force_with_fuel_fun n' h1))
+                | Some h1 \<Rightarrow> force_with_fuel n' h1))
        | _ \<Rightarrow> Some h)"
 
 definition forces_to :: "handle \<Rightarrow> handle \<Rightarrow> bool" where
-  "forces_to h h1 \<equiv> (\<exists>fuel. force_with_fuel_fun fuel h = Some h1 \<and> \<not> is_thunk h1)"
+  "forces_to h h1 \<equiv> (\<exists>fuel. force_with_fuel fuel h = Some h1 \<and> \<not> is_thunk h1)"
 
 (* Determinism *)
 
-lemma step_deterministic:
-  assumes "step op s o1" "step op s o2"
-  shows   "o1 = o2"
-  using assms
-proof (induction arbitrary: o2 rule: step.induct)
-  case (StepGetBlobData i s b)
-  from StepGetBlobData.prems(1) show ?case
-    by (cases rule: step.cases; auto simp: StepGetBlobData(2))
-next
-  case (StepGetTreeData i s b j)
-  from StepGetTreeData.prems(1) show ?case
-    by (cases rule: step.cases; auto simp: StepGetTreeData(2))
-next
-  case (StepCreateBlob i s)
-  from StepCreateBlob.prems(1) show ?case
-    by (cases rule: step.cases; auto)
-next
-  case (StepCreateThunk i s t)
-  from StepCreateThunk.prems(1) show ?case
-    by (cases rule: step.cases; auto simp: StepCreateThunk(2))
-next
-  case (StepCreateTree xs s hs)
-  from StepCreateTree.prems(1) show ?case
-    by (cases rule: step.cases; auto simp: StepCreateTree(2))
-next
-  case (StepReturn i s r)
-  from StepReturn.prems(1) show ?case
-    by (cases rule: step.cases; auto)
-next
-  case (StepRunInternal s)
-  from StepRunInternal.prems(1) show ?case
-    by (cases rule: step.cases; auto)
-qed
-
-lemma exec_deterministic:
-  assumes "exec p s o1" "exec p s o2"
-  shows   "o1 = o2"
-  using assms
-proof (induction arbitrary: o2 rule: exec.induct)
-  case (ExecReturn i s r1 xs)
-  then show ?case
-    by (cases rule: exec.cases[OF ExecReturn.prems(1)])
-      (auto dest: step_deterministic)
-next
-  case (ExecStep i s s' xs r)
-  have H1: "step i s (Continue s')" using ExecStep.hyps(1) by assumption
-  have H2: "exec xs s' r" using ExecStep.hyps(2) by assumption
-  have E2: "exec (i # xs) s o2" using ExecStep.prems by assumption
-
-  then show ?case
-  proof (cases rule: exec.cases[OF E2])
-    case (1 i s r xs)
-    have Hret2: "step i s (Return r)" using 1(4) .
-    have Hret1: "step i s (Continue s')" using 1(1) 1(2) H1 by simp
-    have "Continue s' = Return r" using step_deterministic[OF Hret1 Hret2] by simp
-    thus ?thesis by simp
-  next
-    case (2 ia sa s'a xsa ra)
-    have Hstep1: "step i s (Continue s'a)" using 2(1) 2(2) 2(4) by simp
-    have S: "s' = s'a" using step_deterministic[OF H1 Hstep1] by simp
-    have "exec xs s' o2" using 2(5) 2(1) 2(3) S by auto
-    thus ?thesis using ExecStep.IH by auto
-  qed
-qed
-
-lemma force_with_fuel_deterministic:
-  assumes A: "force_with_fuel n h r1"
-    and B: "force_with_fuel n h r2"
-  shows "r1 = r2"
-  using A B
-proof (induction arbitrary: r2 rule: force_with_fuel.induct)
-  case (Done h n)
-  then show ?case
-    by (cases rule: force_with_fuel.cases[OF Done.prems]) auto
-next
-  case (Step h thunk h1 n h2)
-  then show ?case
-  proof (cases rule: force_with_fuel.cases[OF Step.prems])
-    case (1 ha na)
-    have A: "\<not> is_thunk h" using 1(4) 1(2) by auto
-    have B: "is_thunk h" using local.Step(1) by auto
-    thus ?thesis using A B by auto
-  next
-    case (2 ha thunka h1a na h2a)
-    have "thunka = thunk" using 2(2) 2(4) Step.hyps(1) by auto
-    then have "apply_thunk thunka = apply_thunk thunk" by auto
-    then have "Some h1a = Some h1" using 2(5) Step.hyps(2) by simp
-    then have "h1a = h1" by simp
-    then have "force_with_fuel n h1 h2a" using 2(1) 2(6) by auto
-    thus ?thesis using Step.IH 2(3) by auto
-  qed
-qed
-
-lemma evaluate_with_fuel_pad:
-  assumes "force_with_fuel f h nf" and "\<not> is_thunk nf"
-  shows "force_with_fuel (f + k) h nf"
-  using assms
-  by (induction rule: force_with_fuel.induct) (simp_all add: force_with_fuel.intros)
-
-lemma force_with_fuel_fun_pad:
-  assumes "force_with_fuel_fun f h = Some h1" and "\<not> is_thunk h1"
-  shows "force_with_fuel_fun (f + k) h = Some h1"
+lemma force_with_fuel_pad:
+  assumes "force_with_fuel f h = Some h1" and "\<not> is_thunk h1"
+  shows "force_with_fuel (f + k) h = Some h1"
   using assms
 proof (induction f arbitrary: h)
   case 0 then show ?case by (cases h) auto
@@ -315,21 +168,21 @@ next
   then show ?case 
   proof (cases h) 
     case (HBlobHandle b)
-    then have "force_with_fuel_fun (Suc f') h = Some h" by simp_all
+    then have "force_with_fuel (Suc f') h = Some h" by simp_all
     then have "h1 = h" using Suc.prems(1) by auto
     then show ?thesis using HBlobHandle by auto
   next
     case (HTreeHandle t)
-    then have "force_with_fuel_fun (Suc f') h = Some h" by simp_all
+    then have "force_with_fuel (Suc f') h = Some h" by simp_all
     then have "h1 = h" using Suc.prems(1) by auto
     then show ?thesis using HTreeHandle by auto
   next
     case (HThunkHandle th)
     from Suc.prems(1) HThunkHandle obtain h2 where
-      A: "apply_thunk th = Some h2"
-      and B: "force_with_fuel_fun f' h2 = Some h1" by (simp split: option.splits)
+      A: "think th = Some h2"
+      and B: "force_with_fuel f' h2 = Some h1" by (simp split: option.splits)
 
-    have "force_with_fuel_fun (f' + k) h2 = Some h1" using B Suc.IH Suc.prems(2) by auto
+    have "force_with_fuel (f' + k) h2 = Some h1" using B Suc.IH Suc.prems(2) by auto
     then show ?thesis using HThunkHandle A by simp_all
   qed
 qed
@@ -339,19 +192,19 @@ lemma forces_to_deterministic:
   shows "h1 = h2"
   using assms
 proof -
-  obtain f1 where A: "force_with_fuel_fun f1 h = Some h1" and NT1: "\<not> is_thunk h1"
+  obtain f1 where A: "force_with_fuel f1 h = Some h1" and NT1: "\<not> is_thunk h1"
     using assms(1) unfolding forces_to_def by auto
-  obtain f2 where B: "force_with_fuel_fun f2 h = Some h2" and NT2: "\<not> is_thunk h2"
+  obtain f2 where B: "force_with_fuel f2 h = Some h2" and NT2: "\<not> is_thunk h2"
     using assms(2) unfolding forces_to_def by auto
   let ?F = "max f1 f2"
   let ?k1 = "?F - f1"
   let ?k2 = "?F - f2"
-  have "force_with_fuel_fun (f1 + ?k1) h = Some h1"
-    using force_with_fuel_fun_pad[OF A NT1] .
-  then have AA: "force_with_fuel_fun ?F h = Some h1" by simp
-  have "force_with_fuel_fun (f2 + ?k2) h = Some h2" 
-    using force_with_fuel_fun_pad[OF B NT2] .
-  then have BB: "force_with_fuel_fun ?F h = Some h2" by simp
+  have "force_with_fuel (f1 + ?k1) h = Some h1"
+    using force_with_fuel_pad[OF A NT1] .
+  then have AA: "force_with_fuel ?F h = Some h1" by simp
+  have "force_with_fuel (f2 + ?k2) h = Some h2" 
+    using force_with_fuel_pad[OF B NT2] .
+  then have BB: "force_with_fuel ?F h = Some h2" by simp
   show ?thesis using AA BB by simp
 qed
 
@@ -409,60 +262,39 @@ axiomatization where
   "get_tree_raw (create_tree xs) = xs"
   and
   get_thunk_tree_create_thunk[simp]:
-  "get_thunk_tree (create_thunk t) = t"
+  "get_thunk_tree (create_thunk th) = th"
+  and
+  create_thunk_get_thunk_tree[simp]:
+  "create_thunk (get_thunk_tree t) = t"
 
-(* Coupon rules *)
+coinductive eq :: "handle \<Rightarrow> handle \<Rightarrow> bool" where
+  EqBlob:
+  "(get_blob_data b1 = get_blob_data b2) \<Longrightarrow> eq (HBlobHandle b1) (HBlobHandle b2)"
+| EqTree:
+  "list_all2 eq (get_tree_raw t1) (get_tree_raw t2) \<Longrightarrow>
+   eq (HTreeHandle t1) (HTreeHandle t2)"
+| EqThunk:
+  "force (HThunkHandle th1) = Some r1 \<Longrightarrow>
+   force (HThunkHandle th2) = Some r2 \<Longrightarrow>
+    eq r1 r2 \<Longrightarrow>
+   eq (HThunkHandle th1) (HThunkHandle th2)"
+| EqThunkTree:
+   "eq (HTreeHandle (get_thunk_tree th1)) (HTreeHandle (get_thunk_tree th2)) \<Longrightarrow>
+    eq (HThunkHandle th1) (HThunkHandle th2)"
+| EqSelf:
+   "eq h h"
 
-inductive coupon_eq :: "handle \<Rightarrow> handle \<Rightarrow> bool" where
-  Storage:
-  "get_blob_data h1 = get_blob_data h2 \<Longrightarrow> coupon_eq (HBlobHandle h1) (HBlobHandle h2)"
-| Tree:
-  "get_tree_size t1 = get_tree_size t2 \<Longrightarrow>
-     (\<forall> i < get_tree_size t1. coupon_eq (get_tree_data t1 i) (get_tree_data t2 i)) \<Longrightarrow>
-     coupon_eq (HTreeHandle t1) (HTreeHandle t2)"
-| ThunkByTree:
-  "coupon_eq (HTreeHandle (get_thunk_tree th1)) (HTreeHandle (get_thunk_tree th2)) \<Longrightarrow>
-     coupon_eq (HThunkHandle th1) (HThunkHandle th2)"
-| ThunkByEvaluate:
-  "forces_to (HThunkHandle th1) h \<Longrightarrow>
-     forces_to (HThunkHandle th2) h \<Longrightarrow>
-     coupon_eq (HThunkHandle th1) (HThunkHandle th2)"
+axiomatization where
+  get_prog_eq:
+    "eq (HTreeHandle t1) (HTreeHandle t2) \<Longrightarrow> get_prog t1 = get_prog t2"
 
-(* Semantic rules *)
-
-coinductive sem_eq :: "handle \<Rightarrow> handle \<Rightarrow> bool" where
-  SemBlob:
-  "(get_blob_data b1 = get_blob_data b2) \<Longrightarrow> sem_eq (HBlobHandle b1) (HBlobHandle b2)"
-| SemTree:
-  "list_all2 sem_eq (get_tree_raw t1) (get_tree_raw t2) \<Longrightarrow>
-   sem_eq (HTreeHandle t1) (HTreeHandle t2)"
-| SemThunk:
-  "(force (HThunkHandle th1) = Some r1 \<Longrightarrow>
-    force (HThunkHandle th2) = Some r2 \<Longrightarrow>
-     sem_eq r1 r2) \<Longrightarrow>
-   sem_eq (HThunkHandle th1) (HThunkHandle th2)"
-
-coinductive sem_eq_k :: "nat \<Rightarrow> handle \<Rightarrow> handle \<Rightarrow> bool" where
-  SemBlob:
-  "(get_blob_data b1 = get_blob_data b2) \<Longrightarrow> sem_eq_k k (HBlobHandle b1) (HBlobHandle b2)"
-| SemTree:
-  "list_all2 sem_eq (get_tree_raw t1) (get_tree_raw t2) \<Longrightarrow>
-   sem_eq_k k (HTreeHandle t1) (HTreeHandle t2)"
-| SemThunk0:
-  "sem_eq_k 0 (HThunkHandle th1) (HThunkHandle th2)"
-| SemThunkk:
-  "(force (HThunkHandle th1) = Some r1 \<Longrightarrow>
-    force (HThunkHandle th2) = Some r2 \<Longrightarrow>
-     sem_eq_k k r1 r2) \<Longrightarrow>
-   sem_eq_k (Suc k) (HThunkHandle th1) (HThunkHandle th2)"
-
-lemma sem_eq_same_type:
-  assumes "sem_eq h1 h2"
+lemma eq_same_type:
+  assumes "eq h1 h2"
   shows "get_type h1 = get_type h2"
   using assms
-  by (cases rule: sem_eq.cases) auto
+  by (cases rule: eq.cases) auto 
 
-(* sem_eq preserved by thunk application *)
+(* eq preserved by thunk application *)
 
 (* 1. Useful lemmas and definitions *)
 definition relate_opt :: "('a \<Rightarrow> 'b \<Rightarrow> bool) \<Rightarrow> 'a option \<Rightarrow> 'b option \<Rightarrow> bool" where
@@ -470,9 +302,9 @@ definition relate_opt :: "('a \<Rightarrow> 'b \<Rightarrow> bool) \<Rightarrow>
      (case x of None \<Rightarrow> y = None 
      | Some a \<Rightarrow> (\<exists>b. y = Some b \<and> P a b))"
 
-definition sem_eq_state :: "state \<Rightarrow> state \<Rightarrow> bool" where
-  "sem_eq_state s1 s2 \<equiv>
-     list_all2 (\<lambda>h1 h2. sem_eq h1 h2) (hs s1) (hs s2) \<and> ds s1 = ds s2"
+definition eq_state :: "state \<Rightarrow> state \<Rightarrow> bool" where
+  "eq_state s1 s2 \<equiv>
+     list_all2 (\<lambda>h1 h2. eq h1 h2) (hs s1) (hs s2) \<and> ds s1 = ds s2"
 
 lemma list_all2_append:
   assumes "list_all2 P xs ys"
@@ -481,89 +313,963 @@ lemma list_all2_append:
   using assms
   by (induction arbitrary: x y rule: list_all2_induct) simp_all
 
-lemma list_all2_nthD:
-  assumes "list_all2 R xs ys" "i < length xs"
-  shows "i < length ys \<and> R (xs ! i) (ys ! i)"
-  using assms
-  by (auto simp: list_all2_conv_all_nth)
-
-lemma sem_eq_state_hpush:
-  assumes "sem_eq_state s1 s2" and "sem_eq h1 h2"
-  shows "sem_eq_state (hpush s1 h1) (hpush s2 h2)"
-  using assms unfolding sem_eq_state_def hpush_def
+lemma eq_state_hpush:
+  assumes "eq_state s1 s2" and "eq h1 h2"
+  shows "eq_state (hpush s1 h1) (hpush s2 h2)"
+  using assms unfolding eq_state_def hpush_def
   by (auto simp: list_all2_append)
 
-lemma sem_eq_dpush:
-  assumes "sem_eq_state s1 s2" and "d1 = d2"
-  shows "sem_eq_state (dpush s1 d1) (dpush s2 d2)"
-  using assms unfolding sem_eq_state_def dpush_def by auto
+lemma eq_dpush:
+  assumes "eq_state s1 s2" and "d1 = d2"
+  shows "eq_state (dpush s1 d1) (dpush s2 d2)"
+  using assms unfolding eq_state_def dpush_def by auto
 
-lemma sem_eq_same_kind:
-  assumes "sem_eq h1 h2"
-  shows
-    "(\<exists>b1 b2. h1 = HBlobHandle b1 \<and> h2 = HBlobHandle b2) \<or>
-     (\<exists>t1 t2. h1 = HTreeHandle t1 \<and> h2 = HTreeHandle t2) \<or>
-     (\<exists>k1 k2. h1 = HThunkHandle k1 \<and> h2 = HThunkHandle k2)"
+lemma eq_same_kind_blob:
+  assumes "eq (HBlobHandle b1) h2"
+  obtains "b2" where "h2 = HBlobHandle b2"
   using assms
-  by (cases rule: sem_eq.cases) auto
+  by (cases rule: eq.cases) auto
 
-definition rel_step_result :: "step_result \<Rightarrow> step_result \<Rightarrow> bool" where
-  "rel_step_result r1 r2 \<equiv> 
+lemma eq_not_blob:
+  assumes "eq h1 h2"
+  shows "(\<forall>b. h1 \<noteq> HBlobHandle b) \<Longrightarrow> (\<forall>b. h2 \<noteq> HBlobHandle b)"
+  using assms
+  by (cases rule: eq.cases) auto
+
+lemma eq_same_kind_tree:
+  assumes "eq (HTreeHandle t1) h2"
+  obtains "t2" where "h2 = HTreeHandle t2"
+  using assms
+  by (cases rule: eq.cases) auto
+
+lemma eq_not_tree:
+  assumes "eq h1 h2"
+  shows "(\<forall>t. h1 \<noteq> HTreeHandle t) \<Longrightarrow> (\<forall>t. h2 \<noteq> HTreeHandle t)"
+  using assms
+  by (cases rule: eq.cases) auto
+
+lemma eq_same_kind_thunk:
+  assumes "eq (HThunkHandle th1) h2"
+  obtains "th2" where "h2 = HThunkHandle th2"
+  using assms
+  by (cases rule: eq.cases) auto
+
+lemma eq_not_thunk:
+  assumes "eq h1 h2" and "\<not> is_thunk h1"
+  shows   "\<not> is_thunk h2"
+  using assms
+  by (cases h1) auto
+
+lemma eq_state_hs:
+  "eq_state s1 s2 \<Longrightarrow> list_all2 (\<lambda>h1 h2. eq h1 h2) (hs s1) (hs s2)"
+  by (simp add: eq_state_def)
+
+lemma eq_state_ds:
+  "eq_state s1 s2 \<Longrightarrow> (ds s1) = (ds s2)"
+  by (simp add: eq_state_def)
+
+lemma eq_state_hs_same_length:
+  assumes "eq_state s1 s2"
+  shows "length (hs s1) = length (hs s2)"
+  using eq_state_hs[OF assms]
+  by (simp add: list_all2_lengthD)
+
+lemma eq_state_hs_nth:
+  assumes "eq_state s1 s2" "i < length (hs s1)"
+  shows "eq ((hs s1) ! i) ((hs s2)! i) \<and> i < length (hs s2)"
+  using eq_state_hs[OF assms(1)] assms(2)
+  by (simp add: list_all2_conv_all_nth)
+  
+definition eq_step_result :: "step_result option \<Rightarrow> step_result option \<Rightarrow> bool" where
+  "eq_step_result r1 r2 \<equiv> 
    (case (r1, r2) of
-     (Continue s1, Continue s2) \<Rightarrow> sem_eq_state s1 s2
-   | (Return r1, Return r2) \<Rightarrow> sem_eq r1 r2
+     (Some (Continue s1), Some (Continue s2)) \<Rightarrow> eq_state s1 s2
+   | (Some (Return r1), Some (Return r2)) \<Rightarrow> eq r1 r2
+   | (None, None) \<Rightarrow> True
    | (_, _) \<Rightarrow> False)"
 
 (* 2. API functions respect sem_eq *)
-lemma get_blob_data_sem_eq:
-  assumes "sem_eq (HBlobHandle b1) (HBlobHandle b2)"
+lemma get_blob_data_eq:
+  assumes "eq (HBlobHandle b1) (HBlobHandle b2)"
   shows "get_blob_data b1 = get_blob_data b2"
   using assms
-  by (cases rule: sem_eq.cases) auto
+  by (cases rule: eq.cases) auto
 
-lemma sem_eq_tree_children:
-  assumes "sem_eq (HTreeHandle t1) (HTreeHandle t2)"
-  shows "list_all2 sem_eq (get_tree_raw t1) (get_tree_raw t2)"
+lemma eq_refl: "eq h h" 
+  by (rule eq.EqSelf)
+
+lemma eq_tree_children:
+  assumes "eq (HTreeHandle t1) (HTreeHandle t2)"
+  shows "list_all2 eq (get_tree_raw t1) (get_tree_raw t2)"
   using assms
-  by (cases rule: sem_eq.cases) auto
+proof (cases rule: eq.cases)
+  case EqTree
+  then show ?thesis by auto
+next
+  case (EqSelf)
+  then have "get_tree_raw t1 = get_tree_raw t2" by simp
+  then show ?thesis  
+    by (simp add: list_all2_refl eq_refl)
+qed
 
-lemma get_tree_size_sem_eq:
-  assumes "sem_eq (HTreeHandle t1) (HTreeHandle t2)"
+lemma get_tree_size_eq:
+  assumes "eq (HTreeHandle t1) (HTreeHandle t2)"
   shows   "get_tree_size t1 = get_tree_size t2"
-  using sem_eq_tree_children[OF assms]
+  using eq_tree_children[OF assms]
   by (simp add: get_tree_size_def list_all2_lengthD)
 
-lemma get_tree_data_sem_eq:
-  assumes "sem_eq (HTreeHandle t1) (HTreeHandle t2)" and "i < get_tree_size t1"
-  shows "sem_eq (get_tree_data t1 i) (get_tree_data t2 i)"
+lemma get_tree_data_eq:
+  assumes "eq (HTreeHandle t1) (HTreeHandle t2)" and "i < get_tree_size t1"
+  shows "eq (get_tree_data t1 i) (get_tree_data t2 i)"
 proof -
   have A: "i < length (get_tree_raw t1)" using assms(2) get_tree_size_def by auto
-  have "list_all2 sem_eq (get_tree_raw t1) (get_tree_raw t2)" 
-    using sem_eq_tree_children[OF assms(1)] .
-  then have "sem_eq ((get_tree_raw t1) ! i) ((get_tree_raw t2) ! i)" 
+  have "list_all2 eq (get_tree_raw t1) (get_tree_raw t2)" 
+    using eq_tree_children[OF assms(1)] .
+  then have "eq ((get_tree_raw t1) ! i) ((get_tree_raw t2) ! i)" 
     using list_all2_nthD[OF _ A] by auto
   then show ?thesis by (simp add: get_tree_data_def[symmetric]) 
 qed
 
-lemma create_blob_sem_eq:
+lemma create_blob_eq:
   assumes "d1 = d2"
-  shows "sem_eq (HBlobHandle (create_blob d1)) (HBlobHandle (create_blob d2))"
+  shows "eq (HBlobHandle (create_blob d1)) (HBlobHandle (create_blob d2))"
 proof -
   have "get_blob_data (create_blob d1) = get_blob_data (create_blob d2)" 
     using assms by simp_all
-  then show ?thesis by (rule sem_eq.SemBlob) 
+  then show ?thesis by (rule eq.EqBlob) 
 qed
 
-lemma create_tree_sem_eq:
-  assumes "list_all2 sem_eq xs ys"
-  shows "sem_eq (HTreeHandle (create_tree xs)) (HTreeHandle (create_tree ys))"
+lemma create_tree_eq:
+  assumes "list_all2 eq xs ys"
+  shows "eq (HTreeHandle (create_tree xs)) (HTreeHandle (create_tree ys))"
 proof -
-  have "list_all2 sem_eq (get_tree_raw (create_tree xs)) (get_tree_raw (create_tree ys))"
+  have "list_all2 eq (get_tree_raw (create_tree xs)) (get_tree_raw (create_tree ys))"
     using assms by simp_all
-  then show ?thesis by (rule sem_eq.SemTree)
+  then show ?thesis by (rule eq.EqTree)
+qed
+
+lemma create_thunk_eq:
+  assumes "eq (HTreeHandle t1) (HTreeHandle t2)"
+  shows   "eq (HThunkHandle (create_thunk t1)) (HThunkHandle (create_thunk t2))"
+proof -
+  have EQ: "eq (HTreeHandle (get_thunk_tree (create_thunk t1))) (HTreeHandle (get_thunk_tree (create_thunk t2)))"
+    using assms
+    by simp_all
+  then show ?thesis by (rule eq.EqThunkTree)
+qed
+
+lemma run_internal_eq:
+  assumes "eq_state s1 s2"
+  shows "eq_state (run_internal s1) (run_internal s2)"
+proof -
+  have "list_all2 eq (hs s1) (hs s2)" using assms unfolding eq_state_def by simp_all
+  then have HS: "list_all2 eq (hs (run_internal s1)) (hs (run_internal s2))" 
+    using run_internal_hs 
+    by simp
+
+  have DS: "ds s1 = ds s2" using assms unfolding eq_state_def by simp_all
+  have DS': "ds (run_internal s1) = ds (run_internal s2)"
+    using run_internal_ds_equiv[OF DS]
+    by assumption
+
+  show ?thesis using HS DS' eq_state_def by auto
+qed
+
+lemma step_eq_none:
+  assumes "eq_state s1 s2"
+  and "step op s1 = None"
+  shows "step op s2 = None"
+proof -
+  have L: "length (hs s1) = length (hs s2)" using eq_state_hs_same_length[OF assms(1)] .
+  have D: "(ds s1) = (ds s2)" using eq_state_ds[OF assms(1)] .
+
+  show ?thesis
+  proof (cases op)
+    case (OGetBlobData x)
+    show ?thesis 
+    proof (cases "x < length (hs s1)")
+      case False
+      then show ?thesis using L OGetBlobData False by (simp add: step.simps)
+    next 
+      case True
+      then have EQ: "eq ((hs s1) ! x) ((hs s2) !x)" using eq_state_hs_nth[OF assms(1) True] by simp
+      have "\<not> (\<exists>b. (hs s1) ! x = HBlobHandle b)"
+        using True OGetBlobData assms(2)
+        by (auto simp: step.simps split: handle.splits)
+      then have "\<not> (\<exists>b. (hs s2) ! x = HBlobHandle b)"
+        using eq_not_blob EQ
+        by blast
+      then show ?thesis using OGetBlobData True by (auto simp: step.simps split: handle.splits)
+    qed
+  next
+    case (OGetTreeData x y)
+    show ?thesis
+    proof (cases "x < length (hs s1)")
+      case False
+      then show ?thesis using L OGetTreeData False by (simp add: step.simps)
+    next
+      case True
+      then have EQ: "eq ((hs s1) ! x) ((hs s2) !x)" 
+        using eq_state_hs_nth[OF assms(1) True] by simp
+      have EQL: "x < length (hs s2)" using eq_state_hs_nth[OF assms(1) True] by simp
+      show ?thesis
+      proof (cases "\<not>(\<exists>t. (hs s1) ! x = HTreeHandle t)")
+        case True
+        then have "\<not>(\<exists>t. (hs s2) ! x = HTreeHandle t)" using eq_not_tree EQ by blast
+        then show ?thesis using OGetTreeData True 
+          by (auto simp: step.simps split: handle.splits)
+      next
+        case False
+        then obtain "t1" where EQ1: "(hs s1) ! x = HTreeHandle t1"
+          by auto
+        then have Y: "\<not> y < get_tree_size t1" using OGetTreeData True False assms(2) 
+          by (auto simp add: step.simps split: handle.splits)
+        have "\<exists>t. (hs s2) ! x = HTreeHandle t" using EQ eq_same_kind_tree EQ1 by simp blast
+        then obtain "t2" where EQ2: "(hs s2) ! x = HTreeHandle t2" by auto
+        then have "\<not> y < get_tree_size t2" using Y EQ EQ1 EQ2 get_tree_size_eq by simp
+        then show ?thesis using OGetTreeData EQ2 EQL 
+          by (auto simp: step.simps split: handle.splits)
+      qed
+    qed
+  next
+    case (OCreateBlob x)
+    then show ?thesis using assms(2) OCreateBlob D by (auto simp: step.simps)
+  next
+    case (OCreateThunk x)
+    show ?thesis 
+    proof (cases "x < length (hs s1)")
+      case True
+      have "\<not>(\<exists>t. (hs s1) ! x = HTreeHandle t)" 
+        using eq_state_hs_nth[OF assms(1) True] OCreateThunk True assms(2) 
+        by (auto simp: step.simps split: handle.splits)
+      then have "\<not>(\<exists>t. (hs s2) !x = HTreeHandle t)" 
+        using eq_state_hs_nth[OF assms(1) True] eq_not_tree by auto
+      then show ?thesis using OCreateThunk True 
+        by (auto simp: step.simps split: handle.splits)
+    next 
+      case False
+      then show ?thesis 
+        using L OCreateThunk 
+        by (auto simp: step.simps split: handle.splits)
+    qed
+  next
+    case (OCreateTree xs)
+    then show ?thesis
+      using assms(2) L
+      by (auto simp: step.simps Let_def split: if_splits)
+  next
+    case (ORunInternal)
+    then show ?thesis using assms by (auto simp: step.simps)
+  next
+    case (OReturn x)
+    then show ?thesis using assms L 
+      by (auto simp: step.simps)
+  qed
 qed
 
 
+lemma step_eq_return:
+  assumes "eq_state s1 s2"
+  and "step op s1 = Some (Return h1)"
+shows "\<exists>h2. step op s2 = Some (Return h2) \<and> eq h1 h2"
+proof -
+  have L: "length (hs s1) = length (hs s2)" using eq_state_hs_same_length[OF assms(1)] .
 
+  show ?thesis
+  proof (cases op)
+    case (OGetBlobData x)
+    then have False 
+      using assms(2)
+      by (auto simp: step.simps split: handle.splits if_splits)
+    then show ?thesis by auto
+  next
+    case (OGetTreeData x y)
+    then have False 
+      using assms(2)
+      by (auto simp: step.simps split: handle.splits if_splits)
+    then show ?thesis by auto
+  next
+    case (OCreateBlob x)
+    then have False 
+      using assms(2)
+      by (auto simp: step.simps split: handle.splits if_splits)
+    then show ?thesis by auto
+  next
+    case (OCreateTree xs)
+    then have False 
+      using assms(2)
+      by (auto simp: step.simps split: handle.splits if_splits)
+    then show ?thesis by auto
+  next
+    case (OCreateThunk x)
+    then have False 
+      using assms(2)
+      by (auto simp: step.simps split: handle.splits if_splits)
+    then show ?thesis by auto
+  next
+    case (ORunInternal)
+    then have False 
+      using assms(2)
+      by (auto simp: step.simps split: handle.splits if_splits)
+    then show ?thesis by auto
+  next
+    case (OReturn x)
+    then have L1:"x < length (hs s1)" and H1:"(hs s1) ! x = h1"
+      using assms(2) OReturn
+      by (auto simp: step.simps split: if_splits)
 
+    let ?h2 = "(hs s2) ! x"
+
+    have "x < length (hs s2)" using L L1 by simp
+    then have STEP: "step op s2 = Some (Return ?h2)" 
+      using OReturn 
+      by (auto simp: step.simps)
+
+    have "eq h1 ?h2" using assms(1) H1 eq_state_hs_nth L L1 by auto
+
+    then show ?thesis using STEP by auto
+  qed
+qed
+
+lemma step_eq_continue:
+  assumes "eq_state s1 s2"
+  and "step op s1 = Some (Continue r1)"
+shows "\<exists>r2. step op s2 = Some (Continue r2) \<and> eq_state r1 r2"
+proof -
+  have L: "length (hs s1) = length (hs s2)" using eq_state_hs_same_length[OF assms(1)] .
+  have D : "(ds s1) = (ds s2)" using eq_state_ds[OF assms(1)] .
+
+  show ?thesis
+  proof (cases op)
+    case (OReturn x)
+    then have False 
+      using assms(2)
+      by (cases "x < length (hs s1)") (auto simp: step.simps)
+    then show ?thesis by auto
+  next
+    case (OGetBlobData x)
+    obtain b1 where L1: "x < length (hs s1)" 
+           and B1: "hs s1 ! x = HBlobHandle b1"
+           and R1: "r1 = dpush s1 (get_blob_data b1)"
+      using OGetBlobData assms(2)
+      by (auto simp: step.simps split: if_splits handle.splits step_result.splits)
+
+    have EQ: "eq (hs s1 ! x) (hs s2 ! x)" using L1 assms(1) eq_state_hs_nth by auto
+    then obtain b2 where B2: "hs s2 ! x = HBlobHandle b2" 
+      using eq_same_kind_blob B1 by auto
+
+    have "get_blob_data b1 = get_blob_data b2"
+      using EQ B1 B2 get_blob_data_eq
+      by auto
+
+    then have STATE:"eq_state (dpush s1 (get_blob_data b1)) (dpush s2 (get_blob_data b2))"
+      using assms(1) eq_dpush by auto
+
+    have STEP: "step op s2 = Some(Continue(dpush s2 (get_blob_data b2)))"
+      using L L1 B2 OGetBlobData 
+      by (auto simp: step.simps split:if_splits handle.splits)
+
+    let ?r2 = "Some(Continue(dpush s2 (get_blob_data b2)))"
+    show ?thesis using STEP STATE R1 by auto
+  next
+    case (OGetTreeData x y)
+    obtain h1 where L1: "x < length (hs s1)" 
+              and H1: "hs s1 ! x = HTreeHandle h1" 
+              and S1: "y < get_tree_size h1" 
+              and R1: "r1 = hpush s1 (get_tree_data h1 y)"
+      using assms(2) OGetTreeData by (auto simp: step.simps split: if_splits handle.splits)
+
+    have EQ: "eq (hs s1 ! x) (hs s2 ! x)" using L1 assms(1) eq_state_hs_nth by auto
+    then obtain h2 where H2: "hs s2 ! x = HTreeHandle h2" 
+      using eq_same_kind_tree H1 by auto
+
+    have S2: "y < get_tree_size h2" using EQ H1 H2 get_tree_size_eq S1 by auto
+
+    have EQOUT: "eq (get_tree_data h1 y) (get_tree_data h2 y)" 
+      using get_tree_data_eq S1 EQ H1 H2 by auto
+
+    let ?r2 = "hpush s2 (get_tree_data h2 y)"
+    have STATE: "eq_state r1 ?r2" using eq_state_hpush assms(1) EQOUT S1 R1 by auto
+    have STEP: "step op s2 = Some(Continue ?r2)" using OGetTreeData L L1 H2 S2 
+      by (auto simp: step.simps split: if_splits handle.splits)
+    show ?thesis using STATE STEP by auto
+  next
+    case (OCreateBlob x)
+    then have L1: "x < length (ds s1)" 
+         and R1: "r1 = hpush s1 (HBlobHandle (create_blob (ds s1 ! x)))"
+      using assms(2) by (auto simp: step.simps split: if_splits)
+
+    have "(ds s1) ! x = (ds s2) ! x"
+      using D L1 by simp
+    then have EQOUT: "eq (HBlobHandle (create_blob (ds s1 ! x))) (HBlobHandle (create_blob (ds s2 ! x)))"
+      using create_blob_eq
+      by auto
+
+    let ?r2 = "hpush s2 (HBlobHandle (create_blob (ds s2 ! x)))"
+    have STATE: "eq_state r1 ?r2"
+      using assms(1) EQOUT eq_state_hpush R1 by auto
+    have STEP: "step op s2 = Some (Continue ?r2)"
+      using D L1 OCreateBlob by (auto simp: step.simps split: if_split handle.splits)
+    show ?thesis using STATE STEP by auto
+  next
+    case (OCreateTree xs)
+    let ?hlist1 = "map (\<lambda>i. hs s1 ! i) xs"
+    let ?hlist2 = "map (\<lambda>i. hs s2 ! i) xs"
+
+    have L1: "\<forall>x \<in> set xs. x < length (hs s1)"
+     and R1: "r1 = hpush s1 (HTreeHandle (create_tree ?hlist1))"
+      using assms(2) OCreateTree 
+      by (auto simp: step.simps split: if_splits handle.splits)
+
+    have "list_all2 eq ?hlist1 ?hlist2"
+    proof -
+      have "\<forall> x \<in> set xs. eq (hs s1 ! x) (hs s2 ! x)"
+        using L L1 assms(1) eq_state_hs_nth by auto
+      then show ?thesis by (induction xs) auto
+    qed
+
+    then have EQ: "eq (HTreeHandle (create_tree ?hlist1)) (HTreeHandle (create_tree ?hlist2))"
+      using create_tree_eq
+      by auto
+
+    let ?r2 = "hpush s2 (HTreeHandle (create_tree ?hlist2))"
+    have STATE: "eq_state r1 ?r2"
+      using assms(1) EQ eq_state_hpush R1 by auto
+    have STEP: "step op s2 = Some (Continue ?r2)"
+      using L L1 OCreateTree by (auto simp: step.simps split: if_split handle.splits)
+    show ?thesis using STATE STEP by auto
+  next
+    case (OCreateThunk i)
+    then obtain t1 where L1: "i < length (hs s1)"
+                    and T1: "(hs s1 ! i) = HTreeHandle t1"
+                    and R1: "r1 = hpush s1 (HThunkHandle (create_thunk t1))"
+      using assms(2)
+      by (auto simp: step.simps split: if_splits handle.splits)
+
+    have EQ: "eq (hs s1 ! i) (hs s2 ! i)" 
+      using assms(1) eq_state_hs_nth L L1
+      by auto
+    then obtain t2 where T2: "(hs s2 ! i) = HTreeHandle t2"
+      using eq_same_kind_tree T1
+      by auto
+
+    let ?r2 = "hpush s2 (HThunkHandle (create_thunk t2))"
+
+    have "eq (HThunkHandle (create_thunk t1)) (HThunkHandle (create_thunk t2))"
+      using T1 T2 EQ create_thunk_eq
+      by auto
+    then have STATE: "eq_state r1 ?r2"
+      using assms(1) eq_state_hpush R1 by auto
+    have STEP: "step op s2 = Some (Continue ?r2)"
+      using L L1 OCreateThunk T2 by (auto simp: step.simps split: if_split handle.splits)
+    then show ?thesis using STATE by auto
+  next
+    case (ORunInternal)
+    then have R1: "r1 = run_internal s1"
+      using assms(2)
+      by (auto simp: step.simps)
+
+    let ?r2 = "run_internal s2"
+    have STATE: "eq_state r1 ?r2"
+      using assms(1) R1 run_internal_eq
+      by auto
+    have STEP: "step op s2 = Some (Continue ?r2)" 
+      using ORunInternal by (auto simp: step.simps)
+    then show ?thesis using STATE by auto
+  qed
+qed
+
+lemma step_fun_eq:
+  assumes "eq_state s1 s2"
+  shows   "eq_step_result (step op s1) (step op s2)"
+proof (cases "step op s1")
+  case None
+  then show ?thesis using assms eq_step_result_def step_eq_none by auto
+next
+  case (Some r1)
+  show ?thesis
+  proof (cases r1)
+    case (Continue x1)
+    obtain x2 where "step op s2 = Some (Continue x2) \<and> eq_state x1 x2"
+      using assms Some Continue step_eq_continue by blast
+    then show ?thesis using eq_step_result_def Some Continue by auto
+  next
+    case (Return x1)
+    obtain x2 where "step op s2 = Some (Return x2) \<and> eq x1 x2"
+      using assms Some Return step_eq_return by blast
+    then show ?thesis using eq_step_result_def Some Return by auto
+  qed
+qed
+
+lemma exec_eq_some:
+  assumes "eq_state s1 s2"
+      and "exec p s1 = Some h1"
+    shows "\<exists>h2. exec p s2 = Some h2 \<and> eq h1 h2"
+  using assms
+proof (induction p arbitrary: s1 s2 h1)
+  case Nil
+  then show ?case using assms(1) by auto
+next
+  case (Cons op xs)
+  have EQ: "eq_step_result (step op s1) (step op s2)"
+    using assms(1) step_fun_eq Cons by auto
+
+  show ?case
+  proof (cases "step op s1")
+    case None
+    then show ?thesis using assms(2) Cons by auto
+  next
+    case (Some r1)
+    show ?thesis
+    proof (cases r1)
+      case (Continue s1')
+      then have E1: "exec xs s1' = Some h1"
+        using Some Cons by (auto simp: exec.simps)
+
+      have S1: "step op s1 = Some (Continue s1')" 
+        using Some Continue 
+        by simp
+      then obtain s2' where S2: "step op s2 = Some (Continue s2')"
+        using step_eq_continue assms(1) Cons
+        by blast
+
+      have "eq_step_result (step op s1) (step op s2)"
+        using assms(1) step_fun_eq Cons
+        by blast
+      then have "eq_state s1' s2'"
+        unfolding eq_step_result_def
+        using S1 S2
+        by auto
+
+      then obtain h2 where H2: "exec xs s2' = Some h2 \<and> eq h1 h2"
+        using Cons.IH E1 by blast
+      have "exec (op # xs) s2 = Some h2"
+        using Cons S2 H2 by auto
+      then show ?thesis 
+        using H2 by auto
+    next
+      case (Return h1')
+      then have "h1 = h1'" using assms(2) Some Cons by auto
+      then have H1: "step op s1 = Some (Return h1)" 
+        using Some Return by simp
+      then obtain h2 where H2: "step op s2 = Some (Return h2)"
+        using step_eq_return assms(1) Cons
+        by blast
+
+      have "eq_step_result (step op s1) (step op s2)"
+        using assms(1) step_fun_eq Cons
+        by blast
+      then have "eq h1 h2"
+        unfolding eq_step_result_def
+        using H1 H2
+        by auto
+      then show ?thesis using Cons H2 by auto
+    qed
+  qed
+qed
+
+lemma exec_eq_none:
+"eq_state s1 s2 \<Longrightarrow> exec p s1 = None \<Longrightarrow> exec p s2 = None"
+proof (induction p arbitrary: s1 s2)
+  case Nil
+  then show ?case by auto
+next
+  case (Cons op xs)
+  have EQ: "eq_step_result (step op s1) (step op s2)"
+    using step_fun_eq[OF Cons.prems(1)] Cons by auto
+
+  show ?case
+  proof (cases "step op s1")
+    case None
+    then have "step op s1 = None" by simp
+    then have "step op s2 = None" 
+      using step_eq_none Cons.prems(1)
+      by auto
+    then show ?thesis using Cons by auto
+  next
+    case (Some r1)
+    then show ?thesis
+    proof (cases r1)
+      case (Return h1)
+      then show ?thesis using Cons.prems(2) Cons Some by auto
+    next
+      case (Continue s1')
+      then have S1: "step op s1 = Some (Continue s1')" using Some by simp
+      then obtain s2' where S2: "step op s2 = Some(Continue s2')" 
+                        and EQ': "eq_state s1' s2'"
+        using step_eq_continue Cons.prems(1) by blast
+
+      have "exec xs s1' = None"
+        using Cons Some Continue by simp
+      then have "exec xs s2' = None"
+        using EQ' Cons.IH
+        by auto
+      then show ?thesis using Cons S2 by auto
+    qed
+  qed
+qed
+
+lemma state_init_eq:
+  assumes "eq (HTreeHandle t1) (HTreeHandle t2)"
+  shows "eq_state (state_init (create_thunk t1)) (state_init (create_thunk t2))"
+  using assms
+  unfolding state_init_def eq_state_def
+  by simp
+
+lemma think_eq_some:
+  assumes "eq (HTreeHandle t1) (HTreeHandle t2)"
+      and "think (create_thunk t1) = Some r1"
+    shows "\<exists>r2. think (create_thunk t2) = Some r2 \<and> eq r1 r2"
+proof -
+  let ?s1 = "state_init (create_thunk t1)"
+  let ?s2 = "state_init (create_thunk t2)"
+
+  have EQ: "eq_state ?s1 ?s2"
+    using state_init_eq assms(1)
+    by auto
+
+  have "get_prog (get_thunk_tree (create_thunk t1)) = get_prog (get_thunk_tree (create_thunk t2))"
+    using get_prog_eq assms(1)
+    by auto
+  then have "exec (get_prog (get_thunk_tree (create_thunk t2))) ?s1 = Some r1"
+    using assms(2)
+    unfolding think_def
+    by simp
+  then obtain r2 where "exec (get_prog (get_thunk_tree (create_thunk t2))) ?s2 = Some r2 \<and> eq r1 r2"
+    using EQ exec_eq_some
+    by blast
+  then show ?thesis using think_def by auto
+qed
+
+lemma think_eq_none:
+  assumes "eq (HTreeHandle t1) (HTreeHandle t2)"
+     and "think (create_thunk t1) = None"
+   shows "think (create_thunk t2) = None"
+proof -
+  let ?s1 = "state_init (create_thunk t1)"
+  let ?s2 = "state_init (create_thunk t2)"
+
+  have EQ: "eq_state ?s1 ?s2"
+    using state_init_eq assms(1)
+    by auto
+
+  have "get_prog (get_thunk_tree (create_thunk t1)) = get_prog (get_thunk_tree (create_thunk t2))"
+    using get_prog_eq assms(1)
+    by auto
+  then have "exec (get_prog (get_thunk_tree (create_thunk t2))) ?s1 = None"
+    using assms(2)
+    unfolding think_def
+    by simp
+  then show ?thesis
+    using EQ exec_eq_none think_def
+    by auto
+qed
+
+fun eq_opt :: "handle option \<Rightarrow> handle option \<Rightarrow> bool" where
+  "eq_opt None None = True"
+| "eq_opt (Some h1) (Some h2) = eq h1 h2"
+| "eq_opt _ _ = False"
+
+lemma force_with_fuel_eq:
+  shows "\<And>t1 t2 h1.
+    eq (HTreeHandle t1) (HTreeHandle t2) \<Longrightarrow>
+    force_with_fuel (Suc n1) (HThunkHandle (create_thunk t1)) = Some h1 \<Longrightarrow>
+    \<not> is_thunk h1 \<Longrightarrow>
+    \<exists>n2 h2.
+      force_with_fuel (Suc n2) (HThunkHandle (create_thunk t2)) = Some h2
+      \<and> \<not> is_thunk h2 \<and> eq h1 h2"
+proof (induction n1)
+  case 0
+  then show ?case
+  proof (cases "think (create_thunk t1)")
+    case None
+    then show ?thesis using 0 by auto
+  next
+    case (Some h1')
+    then have "force_with_fuel (Suc 0) (HThunkHandle (create_thunk t1)) = force_with_fuel 0 h1'"
+      using 0 by auto
+    then have "force_with_fuel 0 h1' = Some h1" 
+      using 0 by auto
+    then have NT1: "\<not> is_thunk h1'" and EQ': "Some h1' = Some h1"
+      by (auto simp: force_with_fuel.simps split: if_split handle.splits)
+
+    obtain h2' where Some2: "think (create_thunk t2) = Some h2'"
+                 and    EQ: "eq h1' h2'"
+      using 0(1) think_eq_some Some
+      by blast
+
+    have NT2: "\<not> is_thunk h2'" using NT1 eq_not_thunk EQ by auto
+    then have "force_with_fuel 0 h2' = Some h2'" 
+      by (auto simp: force_with_fuel.simps split: if_split handle.splits)
+    then have FORCE2: "force_with_fuel (Suc 0) (HThunkHandle (create_thunk t2)) = Some h2'"
+      using Some2 by auto
+    have EQN: "eq h1 h2'" using EQ' EQ by simp
+    show ?thesis using FORCE2 NT2 EQN by auto
+  qed
+next
+  case (Suc n)
+  then show ?case
+  proof (cases "think (create_thunk t1)")
+    case None
+    then show ?thesis using Suc by auto
+  next
+    case (Some h1')
+    then have F1: "force_with_fuel (Suc n) h1' = Some h1"
+      using Suc
+      by auto
+
+    show ?thesis
+    proof (cases h1')
+      case (HBlobHandle b1)
+      then have FN1: "force_with_fuel (Suc n) (HThunkHandle (create_thunk t1)) = Some h1'"
+        using Some by auto
+      have NT1: "\<not> is_thunk h1'" using HBlobHandle by auto
+
+      have "force_with_fuel (Suc n) h1' = Some h1'" using HBlobHandle by auto
+      then have EQ1: "h1' = h1" using F1 Suc by auto
+      
+      obtain n2 h2 where FN2: "force_with_fuel (Suc n2) (HThunkHandle (create_thunk t2)) = Some h2"
+                     and NT2: "\<not>is_thunk h2"
+                     and EQ2: "eq h1' h2"
+        using Suc.IH[OF Suc(2) FN1 NT1] by auto
+      have EQ: "eq h1 h2" using EQ1 EQ2 by simp
+      then show ?thesis using FN2 NT2 EQ by auto
+    next
+      case (HTreeHandle tr1)
+      then have FN1: "force_with_fuel (Suc n) (HThunkHandle (create_thunk t1)) = Some h1'"
+        using Some by auto
+      have NT1: "\<not> is_thunk h1'" using HTreeHandle by auto
+
+      have "force_with_fuel (Suc n) h1' = Some h1'" using HTreeHandle by auto
+      then have EQ1: "h1' = h1" using F1 Suc by auto
+      
+      obtain n2 h2 where FN2: "force_with_fuel (Suc n2) (HThunkHandle (create_thunk t2)) = Some h2"
+                     and NT2: "\<not>is_thunk h2"
+                     and EQ2: "eq h1' h2"
+        using Suc.IH[OF Suc(2) FN1 NT1] by auto
+      have EQ: "eq h1 h2" using EQ1 EQ2 by simp
+      then show ?thesis using FN2 NT2 EQ by auto
+    next
+      case (HThunkHandle th1)
+      then have FN1: "force_with_fuel (Suc n) (HThunkHandle th1) = Some h1"
+        using Some Suc by auto
+
+      obtain h2 where T: "think (create_thunk t2) = Some h2"
+                  and E: "eq (HThunkHandle th1) h2"
+        using think_eq_some Suc(2) Some HThunkHandle by blast
+      then obtain th2 where S: "h2 = HThunkHandle th2"
+        using eq_same_kind_thunk by auto
+      then have "think (create_thunk t2) = Some (HThunkHandle th2)" 
+        using T by simp
+      have EQ: "eq (HThunkHandle th1) (HThunkHandle th2)" using S E by simp
+
+      then show ?thesis
+      proof (cases rule: eq.cases)
+        case (EqThunk h1' h2')
+        then have FT: "forces_to (HThunkHandle th2) h2'"
+          using force_some
+          by auto
+        then obtain n2' where "force_with_fuel n2' (HThunkHandle th2) = Some h2'"
+          unfolding forces_to_def
+          by auto
+        then have EV1: "force_with_fuel (Suc n2') (HThunkHandle (create_thunk t2)) = Some h2'"
+          using S T
+          by auto
+
+        from FT have EV2: "\<not> is_thunk h2'" using forces_to_def by auto
+
+        have "\<exists>fuel. force_with_fuel fuel (HThunkHandle th1) = Some h1" 
+          using FN1 by blast
+        then have "forces_to (HThunkHandle th1) h1" using Suc(4) forces_to_def by auto
+        then have "force (HThunkHandle th1) = Some h1" using force_unique by blast
+        then have "h1 = h1'" using EqThunk by simp
+        then have EV3: "eq h1 h2'" using EqThunk by simp
+
+        then show ?thesis using EV1 EV2 EV3 by auto
+      next
+        case (EqThunkTree)
+
+        have "force_with_fuel (Suc n) (HThunkHandle th1) = Some h1"
+          using F1 HThunkHandle by auto
+        then have "force_with_fuel (Suc n) (HThunkHandle (create_thunk (get_thunk_tree th1))) = Some h1"
+          by auto
+        then obtain n2' h2' where F2: "force_with_fuel (Suc n2') (HThunkHandle (create_thunk (get_thunk_tree th2))) = Some h2'"
+                              and NT2: "\<not> is_thunk h2'" 
+                              and EQ2: "eq h1 h2'"
+          using Suc.IH[OF EqThunkTree _ Suc(4)]
+          by auto
+
+        have F2: "force_with_fuel (Suc n2') (HThunkHandle th2) = Some h2'"
+          using F2
+          by simp
+
+        have F2: "force_with_fuel (Suc (Suc n2')) (HThunkHandle (create_thunk t2)) = Some h2'"
+          using F2 T S Suc by auto
+
+        then show ?thesis using F2 NT2 EQ2 by auto
+      next
+        case (EqSelf)
+        then have F2: "force_with_fuel (Suc n) (HThunkHandle th2) = Some h1"
+          using FN1 by simp
+        then have F2: "force_with_fuel (Suc (Suc n)) (HThunkHandle (create_thunk t2)) = Some h1"
+          using T S Suc by auto
+
+        have "eq h1 h1" by (rule eq.EqSelf)
+        then show ?thesis using F2 Suc(4) by auto
+      qed
+    qed
+  qed
+qed
+
+lemma force_eq_tree:
+  assumes "eq (HTreeHandle t1) (HTreeHandle t2)"
+      and "force (HThunkHandle (create_thunk t1)) = Some r1"
+    shows "\<exists>r2. force (HThunkHandle (create_thunk t2)) = Some r2 \<and> eq r1 r2"
+proof -
+  have "forces_to (HThunkHandle (create_thunk t1)) r1"
+    using assms(2) force_some
+    by blast
+  then obtain n1 where F1: "force_with_fuel n1 (HThunkHandle (create_thunk t1)) = Some r1"
+                   and NT1: "\<not> is_thunk r1"
+    using forces_to_def
+    by auto
+
+  show ?thesis
+  proof (cases n1)
+    case 0
+    then show ?thesis using F1 by auto
+  next
+    case (Suc n1')
+    then have "force_with_fuel (Suc n1') (HThunkHandle (create_thunk t1)) = Some r1"
+      using F1 by auto
+    then obtain n2 h2 where F2: "force_with_fuel (Suc n2) (HThunkHandle (create_thunk t2)) = Some h2"
+                        and NT2: "\<not> is_thunk h2"
+                        and EQ2: "eq r1 h2"
+      using force_with_fuel_eq[OF assms(1) _ NT1]
+      by blast
+
+    have "\<exists>n2. force_with_fuel n2 (HThunkHandle (create_thunk t2)) = Some h2" using F2 by blast
+    then have "forces_to (HThunkHandle (create_thunk t2)) h2" using NT2 forces_to_def by blast
+    then have "force (HThunkHandle (create_thunk t2)) = Some h2" using force_unique by auto
+    then show ?thesis using EQ2 by blast
+  qed
+qed
+
+lemma force_to_eq:
+  assumes "eq h1 h2"
+      and "force h1 = Some r1"
+    shows "\<exists>r2. force h2 = Some r2 \<and> eq r1 r2"
+  using assms(1)
+proof (cases rule:eq.cases)
+  case (EqBlob b1 b2)
+  then have "force_with_fuel 0 h1 = Some(HBlobHandle b1)"
+        and "force_with_fuel 0 h2 = Some(HBlobHandle b2)"
+    by auto
+  then have "forces_to h1 (HBlobHandle b1)"
+        and "forces_to h2 (HBlobHandle b2)"
+    using forces_to_def
+    by auto
+  then have F1: "force h1 = Some (HBlobHandle b1)"
+        and F2: "force h2 = Some (HBlobHandle b2)"
+    using force_unique
+    by auto
+
+  have "r1 = HBlobHandle b1" using F1 assms(2) by auto
+  then show ?thesis using assms(1) F2 EqBlob by auto
+next
+  case (EqTree t1 t2)
+  then have "force_with_fuel 0 h1 = Some (HTreeHandle t1)"
+        and "force_with_fuel 0 h2 = Some (HTreeHandle t2)"
+    by auto
+  then have "forces_to h1 (HTreeHandle t1)"
+        and "forces_to h2 (HTreeHandle t2) "
+    using forces_to_def
+    by auto
+  then have F1: "force h1 = Some (HTreeHandle t1)"
+        and F2: "force h2 = Some (HTreeHandle t2)"
+    using force_unique
+    by auto
+
+  have "r1 = HTreeHandle t1" using F1 assms(2) by auto
+  then show ?thesis using assms(1) F2 EqTree by auto
+next
+  case (EqThunk th1 r1' th2 r2')
+  then have F: "force h2 = Some r2'"
+        and E: "eq r1' r2'"
+    by auto
+
+  have "r1 = r1'" using EqThunk assms(2) by auto
+  then have "force h2 = Some r2' \<and> eq r1 r2'" using F E by auto
+  then show ?thesis by auto
+next
+  case (EqSelf)
+  then have X: "force h2 = Some r1" using assms(2) by auto
+  have "eq r1 r1" by (rule eq.EqSelf)
+  then show ?thesis using X by auto
+next
+  case (EqThunkTree th1 th2)
+
+  have F: "force (HThunkHandle (create_thunk (get_thunk_tree th1))) = Some r1"
+    using assms(2) EqThunkTree by simp
+
+  obtain r2 where "force (HThunkHandle (create_thunk (get_thunk_tree th2))) = Some r2 \<and> eq r1 r2"
+    using force_eq_tree[OF EqThunkTree(3) F]  by auto 
+  then have "force (HThunkHandle th2) = Some r2 \<and> eq r1 r2" by simp
+  then show ?thesis using EqThunkTree(2) by simp
+qed
+
+inductive coupon_eq :: "handle \<Rightarrow> handle \<Rightarrow> bool" where
+  CouponBlob:
+  "(get_blob_data b1 = get_blob_data b2) \<Longrightarrow> coupon_eq (HBlobHandle b1) (HBlobHandle b2)"
+| CouponTree:
+  "list_all2 coupon_eq (get_tree_raw t1) (get_tree_raw t2) \<Longrightarrow>
+   coupon_eq (HTreeHandle t1) (HTreeHandle t2)"
+| CouponThunk:
+  "force (HThunkHandle th1) = Some r1 \<Longrightarrow>
+   force (HThunkHandle th2) = Some r2 \<Longrightarrow>
+    coupon_eq r1 r2 \<Longrightarrow>
+   coupon_eq (HThunkHandle th1) (HThunkHandle th2)"
+| CouponThunkTree:
+   "coupon_eq (HTreeHandle (get_thunk_tree th1)) (HTreeHandle (get_thunk_tree th2)) \<Longrightarrow>
+    coupon_eq (HThunkHandle th1) (HThunkHandle th2)"
+| CouponSelf:
+   "coupon_eq h h"
+| CouponThunkForce:
+   "coupon_eq (HThunkHandle th1) (HThunkHandle th2) \<Longrightarrow>
+    force (HThunkHandle th1) = Some r1 \<Longrightarrow>
+    force (HThunkHandle th2) = Some r2 \<Longrightarrow>
+    coupon_eq r1 r2"
+
+theorem coupon_legit:
+  assumes "coupon_eq h1 h2"
+  shows "eq h1 h2"
+  using assms
+proof (induction rule : coupon_eq.induct)
+  case (CouponBlob b1 b2)
+  then show ?case by (rule eq.EqBlob)
+next
+  case (CouponTree t1 t2)
+  then have "list_all2 (\<lambda>x1 x2. eq x1 x2) (get_tree_raw t1) (get_tree_raw t2)"
+    by (induction rule: list_all2_induct) simp_all
+  then show ?case by (rule eq.EqTree)
+next
+  case (CouponThunk th1 r1 th2 r2)
+  show ?case using CouponThunk(1) CouponThunk(2) CouponThunk(4) by (rule eq.EqThunk)
+next
+  case (CouponThunkTree th1 th2)
+  show ?case using CouponThunkTree(2) by (rule eq.EqThunkTree)
+next
+  case (CouponSelf h)
+  show ?case by (rule eq.EqSelf)
+next
+  case (CouponThunkForce th1 th2 r1 r2)
+  then obtain r2' where "force (HThunkHandle th2) = Some r2'"
+                    and "eq r1 r2'"
+    using force_to_eq[OF CouponThunkForce(4)] CouponThunkForce.hyps(2)
+    by auto
+  then have "eq r1 r2" using force_unique CouponThunkForce(3) by auto
+  then show ?case by auto
+qed
+
+end
 
